base.v
@@ -2,6 +2,7 @@ From Coq Require Import Lists.List.
 From Coq Require Import Strings.String.
 From Coq Require Import Arith.
 From VSA Require Import Lattice.
+From VSA Require Import Fixpoints.
 
 Import SetNotations.
 
@@ -88,10 +89,10 @@ Inductive trace: Type :=
 
 Coercion finite_trace_nil : label >-> finite_trace.
 
-Definition at_finite_trace (t : finite_trace) : label :=
+Fixpoint at_finite_trace (t : finite_trace) : label :=
   match t with
   | finite_trace_nil l => l
-  | finite_trace_cons l _ _ => l
+  | finite_trace_cons _ _ t' => at_finite_trace t'
   end.
 
 Definition at_infinite_trace (t : infinite_trace) : label :=
@@ -105,10 +106,10 @@ Definition at_trace (t : trace) : label :=
   | infinite t' => at_infinite_trace t'
   end.
 
-Fixpoint after_finite_trace (t : finite_trace) : label :=
+Definition after_finite_trace (t : finite_trace) : label :=
   match t with
   | finite_trace_nil l => l
-  | finite_trace_cons _ _ t' => after_finite_trace t'
+  | finite_trace_cons l _ _ => l
   end.
 
 Notation "'at⟦' S ⟧" := (at_stmt S).
@@ -116,18 +117,19 @@ Notation "'at⟦' π '⟧t'" := (at_finite_trace π).
 Notation "'after⟦' π '⟧t'" := (after_finite_trace π).
 
 Program Fixpoint concat_finite (t1 t2: finite_trace) {_: after⟦t1⟧t = at⟦t2⟧t}: finite_trace :=
-  match t1 with
-  | finite_trace_nil _ => t2
-  | finite_trace_cons l a t1' => finite_trace_cons l a (@concat_finite t1' t2 _)
+  match t2 with
+  | finite_trace_nil _ => t1
+  | finite_trace_cons l a t2' => finite_trace_cons l a (@concat_finite t1 t2' _)
   end.
 
 Notation "t1 ⁀ t2" := (concat_finite t1 t2) (at level 40).
-Notation "l ⟶( a ) π" := (finite_trace_cons l a π) (at level 50).
+Notation "π ⟶( a ) l" := (finite_trace_cons l a π) (at level 50).
 
 Program Fixpoint concat_infinite (t1: finite_trace) (t2: infinite_trace) {_: after⟦t1⟧t = at_infinite_trace t2}: infinite_trace :=
   match t1 with
   | finite_trace_nil _ => t2
-  | finite_trace_cons l a t1' => infinite_trace_cons l a (@concat_infinite t1' t2 _)
+  | finite_trace_cons _ a t1' =>
+      @concat_infinite t1' (infinite_trace_cons after⟦t1'⟧t a t2) _
   end.
 
 Program Definition concat (t1 t2: trace) : option trace :=
@@ -141,37 +143,43 @@ Program Definition concat (t1 t2: trace) : option trace :=
   | infinite _, _ => Some t1
   end.
 
-Definition value_of (t: finite_trace) (v: variable) : value :=
-  let f :=
-    (fix f (t: finite_trace) : option value :=
-       match t with
-       | finite_trace_nil _ => None
-       | finite_trace_cons _ (TAssign s' _ val') t' =>
-            match f t' with
-            | Some val => Some val
-            | None => if String.eqb v s' then Some val' else None
-            end
-       | finite_trace_cons _ _ t' => f t'
-       end
-    )
-  in
-  match f t with
-  | Some v => v
-  | None => 0
+Fixpoint value_of (t: finite_trace) (v: variable) : value :=
+  match t with
+  | finite_trace_nil _ => 0
+  | finite_trace_cons _ (TAssign s' _ val) t' =>
+      if String.eqb v s' then val else value_of t' v
+  | finite_trace_cons _ _ t' => value_of t' v
   end.
 
 Notation "'ϱ(' π ')'" := (value_of π).
 
-Inductive deductive_prefix_trace_semantics (l': label) (π: finite_trace): stmt -> ℘ finite_trace :=
+(* l' is the label after the statement, and it is not necessarily the label at the end of the traces *)
+Inductive deductive_prefix_trace_semantics (l': label): stmt -> finite_trace -> ℘ finite_trace :=
   | dpts_stmt :
-    forall S, at⟦S⟧ = after⟦π⟧t -> deductive_prefix_trace_semantics l' π S after⟦π⟧t
+    forall S π1, at⟦S⟧ = after⟦π1⟧t -> deductive_prefix_trace_semantics l' S π1 after⟦π1⟧t
   | dpts_assign :
-    forall x a, deductive_prefix_trace_semantics l' π (SAssign after⟦π⟧t x a) (after⟦π⟧t ⟶(TAssign x a (A⟦a⟧ϱ(π))) l')
+    forall x a π1, deductive_prefix_trace_semantics l' (SAssign after⟦π1⟧t x a) π1 (after⟦π1⟧t ⟶(TAssign x a (A⟦a⟧ϱ(π1))) l')
   | dpts_while_false :
-    forall b S π' (H: after⟦π⟧t = at⟦π'⟧t), after⟦π⟧t = after⟦π'⟧t -> B⟦b⟧ϱ(@concat_finite π π' H) = false ->
-      deductive_prefix_trace_semantics l' π (SWhile after⟦π⟧t b S) (after⟦π⟧t ⟶(TBInvalid b) l').
+    forall b S π1 π2 (H: after⟦π1⟧t = at⟦π2⟧t), after⟦π1⟧t = after⟦π2⟧t -> B⟦b⟧ϱ(@concat_finite π1 π2 H) = false ->
+      deductive_prefix_trace_semantics l' (SWhile after⟦π1⟧t b S) π1 (after⟦π1⟧t ⟶(TBInvalid b) l')
+  | dpts_while_true :
+    forall b S π1 π2 π3 (H1: after⟦π1⟧t = at⟦π2⟧t) (H2: at⟦S⟧ = at⟦π3⟧t), after⟦π1⟧t = after⟦π2⟧t ->
+      B⟦b⟧ϱ(@concat_finite π1 π2 H1) = true ->
+      deductive_prefix_trace_semantics after⟦π1⟧t S ((@concat_finite π1 π2 H1) ⟶(TBValid b) at⟦S⟧) π3 ->
+      deductive_prefix_trace_semantics l' (SWhile after⟦π1⟧t b S) π1 (@concat_finite (π2 ⟶(TBValid b) at⟦S⟧) π3 H2).
 
-Definition fixpoint_prefix_trace_semantics (l': label) (π: finite_trace) (S: stmt): ℘ finite_trace :=
+Axiom F_while : (finite_trace -> ℘ finite_trace) -> (finite_trace -> ℘ finite_trace).
+Axiom wp_finite_trace_Ord : Ord (finite_trace -> ℘ finite_trace).
+Axiom wp_finite_trace_Join : Join (finite_trace -> ℘ finite_trace).
+Axiom wp_finite_trace_Meet : Meet (finite_trace -> ℘ finite_trace).
+Definition wp_finite_trace_Top : Top (finite_trace -> ℘ finite_trace) := (fun _ _ => True).
+Definition wp_finite_trace_Bottom : Bottom (finite_trace -> ℘ finite_trace) := (fun _ => ∅).
+Axiom wp_finite_trace_CompleteLattice : @CompleteLattice (finite_trace -> ℘ finite_trace) wp_finite_trace_Ord wp_finite_trace_Join wp_finite_trace_Meet (fun _ _ => True) (fun _ => ∅).
+Print wp_finite_trace_CompleteLattice.
+Definition wp_finite_trace_Poset: Lattice (finite_trace -> ℘ finite_trace) := complete_lattice_lattice wp_finite_trace_CompleteLattice.
+Axiom F_while_Increasing : @Increasing _ _ F_while wp_finite_trace_Ord wp_finite_trace_CompleteLattice.
+
+Definition fixpoint_prefix_trace_semantics (l': label) (S: stmt) (π: finite_trace): ℘ finite_trace :=
   let l := after⟦π⟧t in
   if (Nat.eqb at⟦S⟧ l) then
     match S with
